Updates.

FOL/Definition.lean
@@ -18,7 +18,7 @@ structure Definition : Type :=
 deriving DecidableEq
 
 
-def Env : Type := List Definition
+abbrev Env : Type := List Definition
 
 instance : Membership Definition Env :=
   inferInstanceAs (Membership Definition (List Definition))
